swich into 256 bits created some issues

dfy_model/d0inv.dfy
@@ -5,11 +5,11 @@ module d0inv {
     import opened NativeTypes
     import opened Powers
 
-    method d0inv(w28: uint32)
+    method d0inv(w28: uint256)
         requires w28 % 2 == 1;
     {
-        var w0: uint32 := 2;
-        var w29 : uint32 := 1;
+        var w0: uint256 := 2;
+        var w29 : uint256 := 1;
         var i := 1;
         
         assert (w29 * w28) % power(2, i) == 1 
@@ -17,71 +17,78 @@ module d0inv {
             reveal power();
         }
 
-        while i < 32
-            invariant 1 <= i <= 32;
+
+        while i < 256
+            invariant 1 <= i <= 256;
             invariant (w29 * w28) % power(2, i) == 1;
-            invariant i != 32 ==> w0 == power(2, i);
-            decreases 32 - i;
+            invariant i != 256 ==> w0 == power(2, i);
+            decreases 256 - i;
         {
-            var w1 :uint32 := (w28 * w29) % UINT32_MAX;
+            var w1 :uint256 := (w28 * w29) % UINT256_MAX;
 
             ghost var p := w1;
             ghost var w29_old := w29;
 
-            w1 := (w1 as bv32 & w0 as bv32) as uint32;
-            w29 := (w29 as bv32 | w1 as bv32) as uint32;
+            w1 := (w1 as bv256 & w0 as bv256) as uint256;
+            w29 := (w29 as bv256 | w1 as bv256) as uint256;
 
             and_single_bit_lemma(p, w1, w0, i);
+    
 
             if w1 == 0 {
                 or_zero_nop_lemma(w29_old, w1);
+
+                // assert w0 == power(2, i);
+                // assume (w28 * w29) % w0 == 1;
+                // assume ((w28 * w29) % UINT256_MAX) as bv256 & w0 as bv256 == 0;
                 // assert w29_old == w29;
+                assume false;
                 d0inv_bv_lemma_1(w28 * w29, w0, i);
             } else {
                 assume w29 == w29_old + w0;
                 assert w1 == w0;
 
-                // assert p == (w28 * w29_old) % UINT32_MAX;
-                // assert (p as bv32 & w0 as bv32) as uint32 == w0;
-                d0inv_aux_lemma(p, w29, w29_old, w28, w0, i);
+                // assert p == (w28 * w29_old) % uint256_MAX;
+                // assert (p as bv256 & w0 as bv256) as uint256 == w0;
+                d0inv_aux_lemma_2(p, w29, w29_old, w28, w0, i);
             }
 
-            if i != 31 {
+            if i != 255 {
                 power_2_bounded_lemma(i + 1);
             }
 
-            w0 := if i != 31 then power(2, i + 1) else 0;
+            w0 := if i != 255 then power(2, i + 1) else 0;
             i := i + 1;
-            assert i != 32 ==> w0 == power(2, i);
+            assert i != 256 ==> w0 == power(2, i);
         }
 
-        assert (w29 * w28) % power(2, 32) == 1;
+        assert (w29 * w28) % power(2, 256) == 1;
     }
 
-    lemma {:axiom} and_single_bit_lemma(x: uint32, x': uint32, w0: uint32, i: nat)
+    lemma {:axiom} and_single_bit_lemma(x: uint256, x': uint256, w0: uint256, i: nat)
         requires w0 == power(2, i);
-        requires x' == (x as bv32 & w0 as bv32) as uint32;
+        requires x' == (x as bv256 & w0 as bv256) as uint256;
         ensures x' == power(2, i) || x' == 0;
 
-    lemma or_zero_nop_lemma(x: uint32, z: uint32)
+    lemma or_zero_nop_lemma(x: uint256, z: uint256)
         requires z == 0;
-        ensures (x as bv32 | z as bv32) as uint32 == x;
+        ensures (x as bv256 | z as bv256) as uint256 == x;
     {
-        assert z as bv32 == 0 by {
-            bv32_uint32_casting(z as bv32, z);
+        assert z as bv256 == 0 by {
+            bv256_uint256_casting(z as bv256, z);
         }
-        assert x as bv32 | z as bv32 == x as bv32;
-        bv32_uint32_casting(x as bv32, x);
+        assert x as bv256 | z as bv256 == x as bv256;
+        bv256_uint256_casting(x as bv256, x);
     }
 
-    lemma d0inv_aux_lemma(p: int, w29: int, w29_old: int, w28: uint32, w0: uint32, i: nat)
+    lemma d0inv_aux_lemma_2(p: int, w29: int, w29_old: int, w28: uint256, w0: uint256, i: nat)
         requires w29 == w29_old + w0;
 
-        requires p == (w28 * w29_old) % UINT32_MAX;
+        requires p == (w28 * w29_old) % UINT256_MAX;
         requires w0 == power(2, i);
         requires w28 % 2 == 1;
         requires w28 * w29_old % w0 == 1;
-        requires (p as bv32 & w0 as bv32) as uint32 == w0;
+        requires (p as bv256 & w0 as bv256) as uint256 == w0;
 
         ensures (w29 * w28) % power(2, i + 1) == 1;
     {
@@ -90,8 +97,8 @@ module d0inv {
         }
 
         assert (w28 * w29_old + w28 * w0) % power(2, i + 1) == 1 by {
-            assert p as bv32 & w0 as bv32 == w0 as bv32 by {
-                bv32_uint32_casting(p as bv32 & w0 as bv32, w0);
+            assert p as bv256 & w0 as bv256 == w0 as bv256 by {
+                bv256_uint256_casting(p as bv256 & w0 as bv256, w0);
             }
             d0inv_bv_lemma_2(w28 * w29_old, w28, w0, i);
         }
@@ -99,30 +106,30 @@ module d0inv {
         assert (w29 * w28) % power(2, i + 1) == 1;
     }
 
-    lemma d0inv_nl_aux_lemma(w29: int, w29_old: int, w28: uint32, w0: uint32)
+    lemma d0inv_nl_aux_lemma(w29: int, w29_old: int, w28: uint256, w0: uint256)
         requires w29 == w29_old + w0;
         ensures w29 * w28 == w28 * w29_old + w28 * w0;
     {
         assert true;
     }
 
-    lemma {:axiom} bv32_uint32_casting(bvx: bv32, uintx: uint32)
-        ensures (bvx as uint32 == uintx) <==> (bvx == uintx as bv32);
+    lemma {:axiom} bv256_uint256_casting(bvx: bv256, uintx: uint256)
+        ensures (bvx as uint256 == uintx) <==> (bvx == uintx as bv256);
 
     lemma power_2_bounded_lemma(i: int)
-        requires 0 <= i < 32;
-        ensures power(2, i) <= UINT32_MAX; 
+        requires 0 <= i < 256;
+        ensures power(2, i) <= UINT256_MAX; 
     
-    lemma {:axiom} d0inv_bv_lemma_1(x: int, w0: uint32, i: nat)
+    lemma {:axiom} d0inv_bv_lemma_1(x: int, w0: uint256, i: nat)
         requires w0 == power(2, i);
         requires x % w0 == 1;
-        requires (x % UINT32_MAX) as bv32 & w0 as bv32 == 0;
+        requires (x % UINT256_MAX) as bv256 & w0 as bv256 == 0;
         ensures x % power(2, i + 1) == 1;
 
-    lemma {:axiom} d0inv_bv_lemma_2(x: int, w28: uint32, w0: uint32, i: nat)
+    lemma {:axiom} d0inv_bv_lemma_2(x: int, w28: uint256, w0: uint256, i: nat)
         requires w0 == power(2, i);
         requires x % w0 == 1;
-        requires ((x % UINT32_MAX) as bv32) & (w0 as bv32) == (w0 as bv32);
+        requires ((x % UINT256_MAX) as bv256) & (w0 as bv256) == (w0 as bv256);
         requires w28 % 2 == 1;
         ensures (x + w28 * w0) % power(2, i + 1) == 1;
 }
